theories/lang/steps_inversion.v
@@ -36,6 +36,25 @@ Section inv.
 Variable (fns: fn_env).
 Implicit Type (e: ectx_language.expr (bor_ectx_lang fns)).
 
+Lemma head_step_fill_tstep K
+  e σ e' σ' ev efs :
+  head_step fns e σ ev e' σ' efs →
+  (fill K e, σ) ~{fns}~> (fill K e', σ').
+Proof. intros ?. by econstructor; econstructor. Qed.
+
+Lemma fill_tstep K e σ e' σ' :
+  (e, σ) ~{fns}~>* (e', σ') →
+  (fill K e, σ) ~{fns}~>* (fill K e', σ').
+Proof.
+  intros ST. remember (e, σ) as x. remember (e', σ') as y.
+  revert x y ST e σ Heqx Heqy.
+  induction 1 as [|? [e1 σ1] ? S1 ? IH]; intros e σ H1 H2; subst; simplify_eq.
+  { constructor 1. }
+  etrans; last by apply IH. clear IH ST.
+  apply rtc_once.
+  inv_tstep. rewrite 2!fill_comp. econstructor. by econstructor.
+Qed.
+
 (** PURE STEP ----------------------------------------------------------------*)
 
 (** BinOp *)
